theories/typing/type.v
@@ -57,6 +57,279 @@ Record simple_type `{typeG Σ} :=
 Existing Instance st_own_persistent.
 Instance: Params (@st_own) 2.
 
+Program Definition ty_of_st `{typeG Σ} (st : simple_type) : type :=
+  {| ty_size := 1; ty_own := st.(st_own);
+     (* [st.(st_own) tid vl] needs to be outside of the fractured
+         borrow, otherwise I do not know how to prove the shr part of
+         [subtype_shr_mono]. *)
+     ty_shr := λ κ tid l,
+               (∃ vl, (&frac{κ} λ q, l ↦∗{q} vl) ∗
+                                                 ▷ st.(st_own) tid vl)%I
+  |}.
+Next Obligation. intros. apply st_size_eq. Qed.
+Next Obligation.
+  iIntros (?? st E κ l tid ??) "#LFT Hmt Hκ".
+  iMod (bor_exists with "LFT Hmt") as (vl) "Hmt". set_solver.
+  iMod (bor_sep with "LFT Hmt") as "[Hmt Hown]". set_solver.
+  iMod (bor_persistent with "LFT Hown") as "[Hown|#H†]". set_solver.
+  - iFrame "Hκ".
+    iMod (bor_fracture with "LFT [Hmt]") as "Hfrac"; by eauto with iFrame.
+  - iExFalso. by iApply (lft_tok_dead with "Hκ").
+Qed.
+Next Obligation.
+  iIntros (?? st κ κ' tid l) "#Hord H".
+  iDestruct "H" as (vl) "[#Hf #Hown]".
+  iExists vl. iFrame "Hown". by iApply (frac_bor_shorten with "Hord").
+Qed.
+
+Coercion ty_of_st : simple_type >-> type.
+
+Delimit Scope lrust_type_scope with T.
+Bind Scope lrust_type_scope with type.
+
+(* OFE and COFE structures on types and simple types. *)
+Section ofe.
+  Context `{typeG Σ}.
+
+  Inductive type_equiv' (ty1 ty2 : type) : Prop :=
+    Type_equiv :
+      ty1.(ty_size) = ty2.(ty_size) →
+      (∀ tid vs, ty1.(ty_own) tid vs ≡ ty2.(ty_own) tid vs) →
+      (∀ κ tid l, ty1.(ty_shr) κ tid l ≡ ty2.(ty_shr) κ tid l) →
+      type_equiv' ty1 ty2.
+  Instance type_equiv : Equiv type := type_equiv'.
+  Inductive type_dist' (n : nat) (ty1 ty2 : type) : Prop :=
+    Type_dist :
+      ty1.(ty_size) = ty2.(ty_size) →
+      (∀ tid vs, ty1.(ty_own) tid vs ≡{n}≡ ty2.(ty_own) tid vs) →
+      (∀ κ tid l, ty1.(ty_shr) κ tid l ≡{n}≡ ty2.(ty_shr) κ tid l) →
+      type_dist' n ty1 ty2.
+  Instance type_dist : Dist type := type_dist'.
+
+  Let T := prodC
+    (prodC natC (thread_id -c> list val -c> iProp Σ))
+    (lft -c> thread_id -c> loc -c> iProp Σ).
+  Let P (x : T) : Prop :=
+    (∀ κ tid l, PersistentP (x.2 κ tid l)) ∧
+    (∀ tid vl, x.1.2 tid vl -∗ ⌜length vl = x.1.1⌝) ∧
+    (∀ E κ l tid q, lftE ⊆ E →
+      lft_ctx -∗ &{κ} (l ↦∗: λ vs, x.1.2 tid vs) -∗
+      q.[κ] ={E}=∗ x.2 κ tid l ∗ q.[κ]) ∧
+    (∀ κ κ' tid l, κ' ⊑ κ -∗ x.2 κ tid l -∗ x.2 κ' tid l).
+
+  Definition type_unpack (ty : type) : T :=
+    (ty.(ty_size), λ tid vl, (ty.(ty_own) tid vl), ty.(ty_shr)).
+  Program Definition type_pack (x : T) (H : P x) : type :=
+    {| ty_size := x.1.1; ty_own tid vl := x.1.2 tid vl; ty_shr := x.2 |}.
+  Solve Obligations with by intros [[??] ?] (?&?&?&?).
+
+  Definition type_ofe_mixin : OfeMixin type.
+  Proof.
+    apply (iso_ofe_mixin type_unpack).
+    - split; [by destruct 1|by intros [[??] ?]; constructor].
+    - split; [by destruct 1|by intros [[??] ?]; constructor].
+  Qed.
+  Canonical Structure typeC : ofeT := OfeT type type_ofe_mixin.
+
+  Global Instance ty_size_ne n : Proper (dist n ==> eq) ty_size.
+  Proof. intros ?? EQ. apply EQ. Qed.
+  Global Instance ty_size_proper : Proper ((≡) ==> eq) ty_size.
+  Proof. intros ?? EQ. apply EQ. Qed.
+  Global Instance ty_own_ne n:
+    Proper (dist n ==> eq ==> eq ==> dist n) ty_own.
+  Proof. intros ?? EQ ??-> ??->. apply EQ. Qed.
+  Global Instance ty_own_proper : Proper ((≡) ==> eq ==> eq ==> (≡)) ty_own.
+  Proof. intros ?? EQ ??-> ??->. apply EQ. Qed.
+  Global Instance ty_shr_ne n :
+    Proper (dist n ==> eq ==> eq ==> eq ==> dist n) ty_shr.
+  Proof. intros ?? EQ ??-> ??-> ??->. apply EQ. Qed.
+  Global Instance ty_shr_proper :
+    Proper ((≡) ==> eq ==> eq ==> eq ==> (≡)) ty_shr.
+  Proof. intros ?? EQ ??-> ??-> ??->. apply EQ. Qed.
+
+  Global Instance type_cofe : Cofe typeC.
+  Proof.
+    apply: (iso_cofe_subtype P type_pack type_unpack).
+    - split; [by destruct 1|by intros [[??] ?]; constructor].
+    - by intros [].
+    - intros ? c. rewrite /P /=. split_and!.
+      (* TODO: Can we do these proofs without effectively going into the model? *)
+      + intros κ tid l. apply uPred.entails_equiv_and, equiv_dist=>n.
+        setoid_rewrite conv_compl; simpl.
+        apply equiv_dist, uPred.entails_equiv_and, ty_shr_persistent.
+      + intros tid vl. apply uPred.entails_equiv_and, equiv_dist=>n.
+        repeat setoid_rewrite conv_compl at 1. simpl.
+        apply equiv_dist, uPred.entails_equiv_and, ty_size_eq.
+      + intros E κ l tid q ?. apply uPred.entails_equiv_and, equiv_dist=>n.
+        setoid_rewrite conv_compl; simpl.
+        by apply equiv_dist, uPred.entails_equiv_and, ty_share.
+      + intros κ κ' tid l. apply uPred.entails_equiv_and, equiv_dist=>n.
+        setoid_rewrite conv_compl; simpl.
+        apply equiv_dist, uPred.entails_equiv_and, ty_shr_mono.
+  Qed.
+
+  Inductive st_equiv' (ty1 ty2 : simple_type) : Prop :=
+    St_equiv :
+      (∀ tid vs, ty1.(ty_own) tid vs ≡ ty2.(ty_own) tid vs) →
+      st_equiv' ty1 ty2.
+  Instance st_equiv : Equiv simple_type := st_equiv'.
+  Inductive st_dist' (n : nat) (ty1 ty2 : simple_type) : Prop :=
+    St_dist :
+      (∀ tid vs, ty1.(ty_own) tid vs ≡{n}≡ (ty2.(ty_own) tid vs)) →
+      st_dist' n ty1 ty2.
+  Instance st_dist : Dist simple_type := st_dist'.
+
+  Definition st_unpack (ty : simple_type) : thread_id -c> list val -c> iProp Σ :=
+    λ tid vl, ty.(ty_own) tid vl.
+
+  Definition st_ofe_mixin : OfeMixin simple_type.
+  Proof.
+    apply (iso_ofe_mixin st_unpack).
+    - split; [by destruct 1|by constructor].
+    - split; [by destruct 1|by constructor].
+  Qed.
+  Canonical Structure stC : ofeT := OfeT simple_type st_ofe_mixin.
+
+  Global Instance st_own_ne n :
+    Proper (dist n ==> eq ==> eq ==> dist n) st_own.
+  Proof. intros ?? EQ ??-> ??->. apply EQ. Qed.
+  Global Instance st_own_proper : Proper ((≡) ==> eq ==> eq ==> (≡)) st_own.
+  Proof. intros ?? EQ ??-> ??->. apply EQ. Qed.
+
+  Global Instance ty_of_st_ne : NonExpansive ty_of_st.
+  Proof.
+    intros n ?? EQ. constructor. done. simpl.
+    - intros tid l. apply EQ.
+    - simpl. intros; repeat f_equiv. apply EQ.
+  Qed.
+  Global Instance ty_of_st_proper : Proper ((≡) ==> (≡)) ty_of_st.
+  Proof. apply (ne_proper _). Qed.
+End ofe.
+
+(** Special metric for type-nonexpansive and Type-contractive functions. *)
+Section type_dist2.
+  Context `{typeG Σ}.
+
+  (* Size and shr are n-equal, but own is only n-1-equal.
+     We need this to express what shr has to satisfy on a Type-NE-function:
+     It may only depend contractively on own. *)
+  (* TODO: Find a better name for this metric. *)
+  Inductive type_dist2 (n : nat) (ty1 ty2 : type) : Prop :=
+    Type_dist2 :
+      ty1.(ty_size) = ty2.(ty_size) →
+      (∀ tid vs, dist_later n (ty1.(ty_own) tid vs) (ty2.(ty_own) tid vs)) →
+      (∀ κ tid l, ty1.(ty_shr) κ tid l ≡{n}≡ ty2.(ty_shr) κ tid l) →
+      type_dist2 n ty1 ty2.
+
+  Global Instance type_dist2_equivalence : Equivalence (type_dist2 n).
+  Proof.
+    constructor.
+    - by constructor.
+    - intros ?? Heq; constructor; symmetry; eapply Heq.
+    - intros ??? Heq1 Heq2; constructor; etrans; (eapply Heq1 || eapply Heq2).
+  Qed.
+
+  Definition type_dist2_later (n : nat) ty1 ty2 : Prop :=
+    match n with O => True | S n => type_dist2 n ty1 ty2 end.
+  Arguments type_dist2_later !_ _ _ /.
+
+  Global Instance type_dist2_later_equivalence n :
+    Equivalence (type_dist2_later n).
+  Proof. destruct n as [|n]. by split. apply type_dist2_equivalence. Qed.
+
+  (* The hierarchy of metrics:
+     dist n → type_dist2 n → dist_later n → type_dist2_later. *)
+  Lemma type_dist_dist2 n ty1 ty2 : dist n ty1 ty2 → type_dist2 n ty1 ty2.
+  Proof. intros EQ. split; intros; try apply dist_dist_later; apply EQ. Qed.
+  Lemma type_dist2_dist_later n ty1 ty2 : type_dist2 n ty1 ty2 → dist_later n ty1 ty2.
+  Proof.
+    intros EQ. destruct n; first done. split; intros; try apply EQ.
+    apply dist_S, EQ.
+  Qed.
+  Lemma type_later_dist2_later n ty1 ty2 : dist_later n ty1 ty2 → type_dist2_later n ty1 ty2.
+  Proof. destruct n; first done. exact: type_dist_dist2. Qed.
+  Lemma type_dist2_dist n ty1 ty2 : type_dist2 (S n) ty1 ty2 → dist n ty1 ty2.
+  Proof. move=>/type_dist2_dist_later. done. Qed.
+  Lemma type_dist2_S n ty1 ty2 : type_dist2 (S n) ty1 ty2 → type_dist2 n ty1 ty2.
+  Proof. intros. apply type_dist_dist2, type_dist2_dist. done. Qed.
+
+  Lemma ty_size_type_dist n : Proper (type_dist2 n ==> eq) ty_size.
+  Proof. intros ?? EQ. apply EQ. Qed.
+  Lemma ty_own_type_dist n:
+    Proper (type_dist2 (S n) ==> eq ==> eq ==> dist n) ty_own.
+  Proof. intros ?? EQ ??-> ??->. apply EQ. Qed.
+  Lemma ty_shr_type_dist n :
+    Proper (type_dist2 n ==> eq ==> eq ==> eq ==> dist n) ty_shr.
+  Proof. intros ?? EQ ??-> ??-> ??->. apply EQ. Qed.
+End type_dist2.
+
+(** Type-nonexpansive and Type-contractive functions. *)
+(* Note that TypeContractive is neither weaker nor stronger than Contractive, because
+   (a) it allows the dependency of own on shr to be non-expansive, and
+   (b) it forces the dependency of shr on own to be doubly-contractive.
+   It would be possible to weaken this so that no double-contractivity is required.
+   However, then it is no longer possible to write TypeContractive as just a
+   Proper, which makes it significantly more annoying to use.
+   For similar reasons, TypeNonExpansive is incomparable to NonExpansive.
+*)
+Notation TypeNonExpansive T := (∀ n, Proper (type_dist2 n ==> type_dist2 n) T).
+Notation TypeContractive T := (∀ n, Proper (type_dist2_later n ==> type_dist2 n) T).
+
+Section type_contractive.
+  Context `{typeG Σ}.
+
+  Lemma type_ne_dist_later T :
+    TypeNonExpansive T → ∀ n, Proper (type_dist2_later n ==> type_dist2_later n) T.
+  Proof. intros Hf [|n]; last exact: Hf. hnf. by intros. Qed.
+
+  (* From the above, it easily follows that TypeNonExpansive functions compose with
+     TypeNonExpansive and with TypeContractive functions. *)
+  Lemma type_ne_ne_compose T1 T2 :
+    TypeNonExpansive T1 → TypeNonExpansive T2 → TypeNonExpansive (T1 ∘ T2).
+  Proof. intros NE1 NE2 ? ???; simpl. apply: NE1. exact: NE2. Qed.
+
+  Lemma type_contractive_compose_right T1 T2 :
+    TypeContractive T1 → TypeNonExpansive T2 → TypeContractive (T1 ∘ T2).
+  Proof. intros HT1 HT2 ? ???. apply: HT1. exact: type_ne_dist_later. Qed.
+
+  Lemma type_contractive_compose_left T1 T2 :
+    TypeNonExpansive T1 → TypeContractive T2 → TypeContractive (T1 ∘ T2).
+  Proof. intros HT1 HT2 ? ???; simpl. apply: HT1. exact: HT2. Qed.
+
+  (* Show some more relationships between properties. *)
+  Lemma type_contractive_type_ne T :
+    TypeContractive T → TypeNonExpansive T.
+  Proof.
+    intros HT ? ???. apply type_dist_dist2, dist_later_dist, type_dist2_dist_later, HT. done.
+  Qed.
+
+  Lemma type_contractive_ne T :
+    TypeContractive T → NonExpansive T.
+  Proof.
+    intros HT ? ???. apply dist_later_dist, type_dist2_dist_later, HT, type_dist_dist2. done.
+  Qed.
+
+  (* Simple types *)
+  Global Instance ty_of_st_type_ne n :
+    Proper (dist_later n ==> type_dist2 n) ty_of_st.
+  Proof.
+    intros ???. constructor.
+    - done.
+    - intros. destruct n; first done; simpl. by f_equiv.
+    - intros. solve_contractive.
+  Qed.
+End type_contractive.
+
+(* Tactic automation. *)
+Ltac f_type_equiv :=
+  first [ ((eapply ty_size_type_dist || eapply ty_shr_type_dist || eapply ty_own_type_dist); try reflexivity) |
+          match goal with | |- @dist_later ?A ?n ?x ?y =>
+                            destruct n as [|n]; [exact I|change (@dist A _ n x y)]
+          end ].
+Ltac solve_type_proper :=
+  constructor;
+  solve_proper_core ltac:(fun _ => f_type_equiv || f_contractive || f_equiv).
+
 Section type.
   Context `{typeG Σ}.
 
@@ -122,54 +395,19 @@ Section type.
   }.
   Global Existing Instances copy_persistent.
 
+  Global Instance copy_equiv :
+    Proper (equiv ==> impl) Copy.
+  Proof.
+    intros ty1 ty2 [EQsz%leibniz_equiv EQown EQshr] Hty1. split.
+    - intros. rewrite -EQown. apply _.
+    - intros *. rewrite -EQsz -EQshr. setoid_rewrite <-EQown.
+      apply copy_shr_acc.
+  Qed.
+
   Class LstCopy (tys : list type) := lst_copy : Forall Copy tys.
   Global Instance lst_copy_nil : LstCopy [] := List.Forall_nil _.
   Global Instance lst_copy_cons ty tys :
     Copy ty → LstCopy tys → LstCopy (ty::tys) := List.Forall_cons _ _ _.
-
-  (** Send and Sync types *)
-  Class Send (t : type) :=
-    send_change_tid tid1 tid2 vl : t.(ty_own) tid1 vl -∗ t.(ty_own) tid2 vl.
-
-  Class LstSend (tys : list type) := lst_send : Forall Send tys.
-  Global Instance lst_send_nil : LstSend [] := List.Forall_nil _.
-  Global Instance lst_send_cons ty tys :
-    Send ty → LstSend tys → LstSend (ty::tys) := List.Forall_cons _ _ _.
-
-  Class Sync (t : type) :=
-    sync_change_tid κ tid1 tid2 l : t.(ty_shr) κ tid1 l -∗ t.(ty_shr) κ tid2 l.
-
-  Class LstSync (tys : list type) := lst_sync : Forall Sync tys.
-  Global Instance lst_sync_nil : LstSync [] := List.Forall_nil _.
-  Global Instance lst_sync_cons ty tys :
-    Sync ty → LstSync tys → LstSync (ty::tys) := List.Forall_cons _ _ _.
-
-  (** Simple types *)
-  Program Definition ty_of_st (st : simple_type) : type :=
-    {| ty_size := 1; ty_own := st.(st_own);
-
-       (* [st.(st_own) tid vl] needs to be outside of the fractured
-          borrow, otherwise I do not know how to prove the shr part of
-          [subtype_shr_mono]. *)
-       ty_shr := λ κ tid l,
-                 (∃ vl, (&frac{κ} λ q, l ↦∗{q} vl) ∗
-                        ▷ st.(st_own) tid vl)%I
-    |}.
-  Next Obligation. intros. apply st_size_eq. Qed.
-  Next Obligation.
-    iIntros (st E κ l tid ??) "#LFT Hmt Hκ".
-    iMod (bor_exists with "LFT Hmt") as (vl) "Hmt". set_solver.
-    iMod (bor_sep with "LFT Hmt") as "[Hmt Hown]". set_solver.
-    iMod (bor_persistent with "LFT Hown") as "[Hown|#H†]". set_solver.
-    - iFrame "Hκ".
-      iMod (bor_fracture with "LFT [Hmt]") as "Hfrac"; by eauto with iFrame.
-    - iExFalso. by iApply (lft_tok_dead with "Hκ").
-  Qed.
-  Next Obligation.
-    intros st κ κ' tid l. iIntros "#Hord H".
-    iDestruct "H" as (vl) "[#Hf #Hown]".
-    iExists vl. iFrame "Hown". by iApply (frac_bor_shorten with "Hord").
-  Qed.
 
   Global Program Instance ty_of_st_copy st : Copy (ty_of_st st).
   Next Obligation.
@@ -188,6 +426,37 @@ Section type.
     iDestruct "Hmt" as "[>% Hmt]". subst. by iApply "Hclose".
   Qed.
 
+  (** Send and Sync types *)
+  Class Send (t : type) :=
+    send_change_tid tid1 tid2 vl : t.(ty_own) tid1 vl -∗ t.(ty_own) tid2 vl.
+
+  Global Instance send_equiv :
+    Proper (equiv ==> impl) Send.
+  Proof.
+    intros ty1 ty2 [EQsz%leibniz_equiv EQown EQshr] Hty1.
+    rewrite /Send=>???. rewrite -!EQown. auto.
+  Qed.
+
+  Class LstSend (tys : list type) := lst_send : Forall Send tys.
+  Global Instance lst_send_nil : LstSend [] := List.Forall_nil _.
+  Global Instance lst_send_cons ty tys :
+    Send ty → LstSend tys → LstSend (ty::tys) := List.Forall_cons _ _ _.
+
+  Class Sync (t : type) :=
+    sync_change_tid κ tid1 tid2 l : t.(ty_shr) κ tid1 l -∗ t.(ty_shr) κ tid2 l.
+
+  Global Instance sync_equiv :
+    Proper (equiv ==> impl) Sync.
+  Proof.
+    intros ty1 ty2 [EQsz%leibniz_equiv EQown EQshr] Hty1.
+    rewrite /Send=>????. rewrite -!EQshr. auto.
+  Qed.
+
+  Class LstSync (tys : list type) := lst_sync : Forall Sync tys.
+  Global Instance lst_sync_nil : LstSync [] := List.Forall_nil _.
+  Global Instance lst_sync_cons ty tys :
+    Sync ty → LstSync tys → LstSync (ty::tys) := List.Forall_cons _ _ _.
+
   Global Instance ty_of_st_sync st :
     Send (ty_of_st st) → Sync (ty_of_st st).
   Proof.
@@ -196,136 +465,18 @@ Section type.
   Qed.
 End type.
 
-Coercion ty_of_st : simple_type >-> type.
-
-Delimit Scope lrust_type_scope with T.
-Bind Scope lrust_type_scope with type.
-
-(* OFE and COFE structures on types and simple types. *)
-Section ofe.
-  Context `{typeG Σ}.
-
-  Inductive type_equiv' (ty1 ty2 : type) : Prop :=
-    Type_equiv :
-      ty1.(ty_size) = ty2.(ty_size) →
-      (∀ tid vs, ty1.(ty_own) tid vs ≡ ty2.(ty_own) tid vs) →
-      (∀ κ tid l, ty1.(ty_shr) κ tid l ≡ ty2.(ty_shr) κ tid l) →
-      type_equiv' ty1 ty2.
-  Instance type_equiv : Equiv type := type_equiv'.
-  Inductive type_dist' (n : nat) (ty1 ty2 : type) : Prop :=
-    Type_dist :
-      ty1.(ty_size) = ty2.(ty_size) →
-      (∀ tid vs, dist_later n (ty1.(ty_own) tid vs) (ty2.(ty_own) tid vs)) →
-      (∀ κ tid l, ty1.(ty_shr) κ tid l ≡{n}≡ ty2.(ty_shr) κ tid l) →
-      type_dist' n ty1 ty2.
-  Instance type_dist : Dist type := type_dist'.
-
-  Let T := prodC
-    (prodC natC (thread_id -c> list val -c> laterC (iProp Σ)))
-    (lft -c> thread_id -c> loc -c> iProp Σ).
-  Let P (x : T) : Prop :=
-    (∀ κ tid l, PersistentP (x.2 κ tid l)) ∧
-    (∀ tid vl, (later_car (x.1.2 tid vl) : iProp Σ) -∗ ⌜length vl = x.1.1⌝) ∧
-    (∀ E κ l tid q, lftE ⊆ E →
-      lft_ctx -∗ &{κ} (l ↦∗: λ vs, later_car (x.1.2 tid vs)) -∗
-      q.[κ] ={E}=∗ x.2 κ tid l ∗ q.[κ]) ∧
-    (∀ κ κ' tid l, κ' ⊑ κ -∗ x.2 κ tid l -∗ x.2 κ' tid l).
-
-  Definition type_unpack (ty : type) : T :=
-    (ty.(ty_size), λ tid vl, Next (ty.(ty_own) tid vl), ty.(ty_shr)).
-  Program Definition type_pack (x : T) (H : P x) : type :=
-    {| ty_size := x.1.1; ty_own tid vl := later_car (x.1.2 tid vl); ty_shr := x.2 |}.
-  Solve Obligations with by intros [[??] ?] (?&?&?&?).
-
-  Definition type_ofe_mixin : OfeMixin type.
-  Proof.
-    apply (iso_ofe_mixin type_unpack).
-    - split; [by destruct 1|by intros [[??] ?]; constructor].
-    - split; [by destruct 1|by intros [[??] ?]; constructor].
-  Qed.
-  Canonical Structure typeC : ofeT := OfeT type type_ofe_mixin.
-
-  Global Instance ty_size_ne n : Proper (dist n ==> eq) ty_size.
-  Proof. intros ?? EQ. apply EQ. Qed.
-  Global Instance ty_size_proper : Proper ((≡) ==> eq) ty_size.
-  Proof. intros ?? EQ. apply EQ. Qed.
-  Global Instance ty_own_ne n:
-    Proper (dist (S n) ==> eq ==> eq ==> dist n) ty_own.
-  Proof. intros ?? EQ ??-> ??->. apply EQ. Qed.
-  Global Instance ty_own_proper : Proper ((≡) ==> eq ==> eq ==> (≡)) ty_own.
-  Proof. intros ?? EQ ??-> ??->. apply EQ. Qed.
-  Global Instance ty_shr_ne n :
-    Proper (dist n ==> eq ==> eq ==> eq ==> dist n) ty_shr.
-  Proof. intros ?? EQ ??-> ??-> ??->. apply EQ. Qed.
-  Global Instance ty_shr_proper :
-    Proper ((≡) ==> eq ==> eq ==> eq ==> (≡)) ty_shr.
-  Proof. intros ?? EQ ??-> ??-> ??->. apply EQ. Qed.
-
-  Global Instance type_cofe : Cofe typeC.
-  Proof.
-    apply: (iso_cofe_subtype P type_pack type_unpack).
-    - split; [by destruct 1|by intros [[??] ?]; constructor].
-    - by intros [].
-    - intros ? c. rewrite /P /=. split_and!.
-      + intros κ tid l. apply uPred.entails_equiv_and, equiv_dist=>n.
-        setoid_rewrite conv_compl; simpl.
-        apply equiv_dist, uPred.entails_equiv_and, ty_shr_persistent.
-      + intros tid vl. apply uPred.entails_equiv_and, equiv_dist=>n.
-        rewrite !conv_compl /=.
-        apply equiv_dist, uPred.entails_equiv_and, ty_size_eq.
-      + intros E κ l tid q ?. apply uPred.entails_equiv_and, equiv_dist=>n.
-        setoid_rewrite conv_compl; simpl.
-        rewrite -(c.(chain_cauchy) n (S n)); last lia.
-        by apply equiv_dist, uPred.entails_equiv_and, ty_share.
-      + intros κ κ' tid l. apply uPred.entails_equiv_and, equiv_dist=>n.
-        setoid_rewrite conv_compl; simpl.
-        apply equiv_dist, uPred.entails_equiv_and, ty_shr_mono.
-  Qed.
-
-  Inductive st_equiv' (ty1 ty2 : simple_type) : Prop :=
-    St_equiv :
-      (∀ tid vs, ty1.(ty_own) tid vs ≡ ty2.(ty_own) tid vs) →
-      st_equiv' ty1 ty2.
-  Instance st_equiv : Equiv simple_type := st_equiv'.
-  Inductive st_dist' (n : nat) (ty1 ty2 : simple_type) : Prop :=
-    St_dist :
-      (∀ tid vs, dist_later n (ty1.(ty_own) tid vs) (ty2.(ty_own) tid vs)) →
-      st_dist' n ty1 ty2.
-  Instance st_dist : Dist simple_type := st_dist'.
-
-  Definition st_unpack (ty : simple_type) : thread_id -c> list val -c> laterC (iProp Σ) :=
-    λ tid vl, Next (ty.(ty_own) tid vl).
-
-  Definition st_ofe_mixin : OfeMixin simple_type.
-  Proof.
-    apply (iso_ofe_mixin st_unpack).
-    - split; [by destruct 1|by constructor].
-    - split; [by destruct 1|by constructor].
-  Qed.
-  Canonical Structure stC : ofeT := OfeT simple_type st_ofe_mixin.
-
-  Global Instance st_own_ne n :
-    Proper (dist (S n) ==> eq ==> eq ==> dist n) st_own.
-  Proof. intros ?? EQ ??-> ??->. apply EQ. Qed.
-  Global Instance st_own_proper : Proper ((≡) ==> eq ==> eq ==> (≡)) st_own.
-  Proof. intros ?? EQ ??-> ??->. apply EQ. Qed.
-
-  Global Instance ty_of_st_ne : NonExpansive ty_of_st.
-  Proof.
-    intros n ?? EQ. constructor. done. simpl.
-    - intros tid l. apply EQ.
-    - simpl. intros; repeat (f_contractive || f_equiv). apply EQ.
-  Qed.
-  Global Instance ty_of_st_proper : Proper ((≡) ==> (≡)) ty_of_st.
-  Proof. apply (ne_proper _). Qed.
-End ofe.
-
 Section subtyping.
   Context `{typeG Σ}.
   Definition type_incl (ty1 ty2 : type) : iProp Σ :=
     (⌜ty1.(ty_size) = ty2.(ty_size)⌝ ∗
      (□ ∀ tid vl, ty1.(ty_own) tid vl -∗ ty2.(ty_own) tid vl) ∗
      (□ ∀ κ tid l, ty1.(ty_shr) κ tid l -∗ ty2.(ty_shr) κ tid l))%I.
+
+  Global Instance type_incl_ne : NonExpansive2 type_incl.
+  Proof.
+    intros n ?? [EQsz1%leibniz_equiv EQown1 EQshr1] ?? [EQsz2%leibniz_equiv EQown2 EQshr2].
+    rewrite /type_incl. repeat ((by auto) || f_equiv).
+  Qed.
 
   Global Instance type_incl_persistent ty1 ty2 : PersistentP (type_incl ty1 ty2) := _.
   (*  Typeclasses Opaque type_incl. *)
@@ -347,9 +498,6 @@ Section subtyping.
 
   Definition subtype (ty1 ty2 : type) : Prop :=
     elctx_interp_0 E -∗ ⌜llctx_interp_0 L⌝ -∗ type_incl ty1 ty2.
-  (* TODO RJ: I'd really like to get rid of this definition. *)
-  Definition ctx_eq {A} (x1 x2 : A) : Prop :=
-    elctx_interp_0 E -∗ ⌜llctx_interp_0 L⌝ -∗ ⌜x1 = x2⌝.
 
   Lemma subtype_refl ty : subtype ty ty.
   Proof. iIntros. iApply type_incl_refl. Qed.
@@ -362,6 +510,10 @@ Section subtyping.
     - iApply (H23 with "[] []"); done.
   Qed.
 
+  (* Conditional equality (intended to be used with sizes) *)
+  (* TODO RJ: I'd really like to get rid of this definition. *)
+  Definition ctx_eq {A} (x1 x2 : A) : Prop :=
+    elctx_interp_0 E -∗ ⌜llctx_interp_0 L⌝ -∗ ⌜x1 = x2⌝.
   Lemma ctx_eq_refl {A} (x : A) : ctx_eq x x.
   Proof. by iIntros "_ _". Qed.
   Global Instance ctx_eq_equivalent {A} : Equivalence (@ctx_eq A).
