theories/typing/sum.v
@@ -95,21 +95,22 @@ Section sum.
     - iApply ((nth i tyl ∅).(ty_shr_mono) with "Hord"); done.
   Qed.
 
-  Global Instance sum_ne n: Proper (dist n ==> dist n) sum.
+  Global Instance sum_type_ne n: Proper (Forall2 (type_dist2 n) ==> type_dist2 n) sum.
   Proof.
     intros x y EQ.
     assert (EQmax : list_max (map ty_size x) = list_max (map ty_size y)).
     { induction EQ as [|???? EQ _ IH]=>//=.
       rewrite IH. f_equiv. apply EQ. }
-    assert (EQnth :∀ i, nth i x ∅ ≡{n}≡ nth i y ∅).
+    (* TODO: If we had the right lemma relating nth, (Forall2 R) and R, we should
+       be able to make this more automatic. *)
+    assert (EQnth :∀ i, type_dist2 n (nth i x ∅) (nth i y ∅)).
     { clear EQmax. induction EQ as [|???? EQ _ IH]=>-[|i] //=. }
     constructor; simpl.
     - by rewrite EQmax.
-    - intros tid vl. destruct n as [|n]=> //=. rewrite EQmax. by setoid_rewrite EQnth.
+    - intros tid vl. destruct n as [|n]=> //=. rewrite EQmax.
+      solve_proper_core ltac:(fun _ => exact:EQnth || f_type_equiv || f_equiv).
     - intros κ tid l. unfold is_pad. rewrite EQmax.
-      assert (EQsz : ∀ i, (nth i x ∅).(ty_size) = (nth i y ∅).(ty_size))
-        by (intros; apply EQnth).
-      repeat (rewrite EQsz || apply EQnth || f_equiv).
+      solve_proper_core ltac:(fun _ => exact:EQnth || f_type_equiv || f_equiv).
   Qed.
 
   Global Instance sum_mono E L :
